coq/NNRCimp/Lang/NNRCImpSemEval.v
@@ -1,0 +1,225 @@
+(*
+ * Copyright 2015-2016 IBM Corporation
+ *
+ * Licensed under the Apache License, Version 2.0 (the "License");
+ * you may not use this file except in compliance with the License.
+ * You may obtain a copy of the License at
+ *
+ * http://www.apache.org/licenses/LICENSE-2.0
+ *
+ * Unless required by applicable law or agreed to in writing, software
+ * distributed under the License is distributed on an "AS IS" BASIS,
+ * WITHOUT WARRANTIES OR CONDITIONS OF ANY KIND, either express or implied.
+ * See the License for the specific language governing permissions and
+ * limitations under the License.
+ *)
+
+(** NNRCimp is a variant of the named nested relational calculus
+     (NNRC) that is meant to be more imperative in feel.  It is used
+     as an intermediate language between NNRC and more imperative /
+     statement oriented backends *)
+
+Section NNRCimpSemEval.
+  Require Import String.
+  Require Import List.
+  Require Import Arith.
+  Require Import EquivDec.
+  Require Import Morphisms.
+  Require Import Arith.
+  Require Import Max.
+  Require Import Bool.
+  Require Import Peano_dec.
+  Require Import EquivDec.
+  Require Import Decidable.
+  Require Import Utils.
+  Require Import CommonRuntime.
+  Require Import NNRCimp.
+  Require Import NNRCimpSem.
+  Require Import NNRCimpEval.
+
+  Context {fruntime:foreign_runtime}.
+
+  Context (h:brand_relation_t).
+  Context (σc:list (string*data)).
+
+  Local Open Scope nnrc_imp.
+  Local Open Scope string.
+
+  Lemma nnrc_imp_expr_sem_eval σ e d :
+    [ h , σc ; σ ⊢ e ⇓ d ] <-> [ h , σc ; σ ⊢〚 e 〛 ] = Some d.
+  Proof.
+    split; revert σ d.
+    - {
+        nnrc_imp_expr_cases (induction e) Case; intros σ d₀ sem; invcs sem; simpl; trivial.
+        - Case "NNRCimpVar".
+          rewrite H1; simpl; reflexivity.
+        - Case "NNRCimpBinop".
+          erewrite IHe1 by eauto.
+          erewrite IHe2 by eauto.
+          simpl; trivial.
+        - Case "NNRCimpUnop".
+          erewrite IHe by eauto.
+          simpl; trivial.
+        - Case "NNRCimpGroupBy".
+          erewrite IHe by eauto.
+          simpl; rewrite H5; simpl; trivial.
+      }
+    - {
+        Hint Constructors nnrc_imp_expr_sem.
+        nnrc_imp_expr_cases (induction e) Case; intros σ d₀ sem; invcs sem; simpl; trivial; eauto 3.
+        - Case "NNRCimpVar".
+          apply some_olift in H0.
+          destruct H0 as [??]; unfold id in *; subst.
+          eauto.
+        - Case "NNRCimpBinop".
+          apply some_olift2 in H0.
+          destruct H0 as [?[?? [??]]].
+          eauto.
+        - Case "NNRCimpUnop".
+          apply some_olift in H0.
+          destruct H0 as [??]; unfold id in *; subst.
+          eauto.
+        - Case "NNRCimpGroupBy".
+          match_case_in H0;
+            [intros ? eqq | intros eqq]; rewrite eqq in H0;
+              try discriminate.
+          destruct d; try discriminate.
+          apply some_olift in H0.
+          destruct H0 as [??]; unfold id in *; subst.
+          invcs e1.
+          eauto.
+      }
+  Qed.
+
+  Ltac destr H :=
+    let eqq := fresh "eqq" in
+    first [(match_case_in H;
+            [intros [??] eqq | intros eqq]; rewrite eqq in H; try discriminate)
+          | (match_case_in H;
+             [intros ? eqq | intros eqq]; rewrite eqq in H; try discriminate)
+          | (match_case_in H;
+             [intros eqq | intros ? ? eqq]; try rewrite eqq in H; try discriminate)
+          | (match_case_in H;
+             [intros eqq | intros ? eqq]; try rewrite eqq in H; try discriminate)
+          ]; subst.
+  
+  Lemma nnrc_imp_stmt_sem_eval σ₁ ψ₁ s σ₂ ψ₂ :
+    [ h , σc ; σ₁, ψ₁ ⊢ s ⇓ σ₂, ψ₂ ] <-> [ h , σc ; σ₁, ψ₁ ⊢〚 s 〛 ] = Some (σ₂, ψ₂).
+  Proof.
+    split; revert σ₁ ψ₁ σ₂ ψ₂.
+    - {
+        nnrc_imp_stmt_cases (induction s) Case; intros σ₁ ψ₁ σ₂ ψ₂ sem; invcs sem; simpl; trivial.
+        - Case "NNRCimpSeq".
+          erewrite IHs1 by eauto.
+          eauto.
+        - Case "NNRCimpLetMut".
+          apply nnrc_imp_expr_sem_eval in H6; rewrite H6.
+          erewrite IHs by eauto.
+          simpl; trivial.
+        - Case "NNRCimpLetMut".
+          erewrite IHs by eauto.
+          simpl; trivial.
+        - Case "NNRCimpBuildCollFor".
+          erewrite IHs1 by eauto; simpl.
+          erewrite IHs2 by eauto; simpl; trivial.
+        - Case "NNRCimpPush".
+          rewrite nnrc_imp_expr_sem_eval in H6; rewrite H6.
+          rewrite H3; simpl; trivial.
+        - Case "NNRCimpAssign".
+          rewrite nnrc_imp_expr_sem_eval in H6; rewrite H6.
+          rewrite H3; simpl; trivial.
+        - Case "NNRCimpFor".
+          rewrite nnrc_imp_expr_sem_eval in H6; rewrite H6; clear H6.
+          revert σ₁ ψ₁ σ₂ ψ₂ H7.
+          induction dl; intros σ₁ ψ₁ σ₂ ψ₂ seval; invcs seval; trivial.
+          erewrite IHs by eauto; simpl.
+          eauto.
+        - Case "NNRCimpIf".
+          rewrite nnrc_imp_expr_sem_eval in H6; rewrite H6.
+          eauto.
+        - Case "NNRCimpIf".
+          rewrite nnrc_imp_expr_sem_eval in H6; rewrite H6.
+          eauto.
+        - Case "NNRCimpEither".
+          rewrite nnrc_imp_expr_sem_eval in H8; rewrite H8.
+          erewrite IHs1 by eauto.
+          simpl; trivial.
+        - Case "NNRCimpEither".
+          rewrite nnrc_imp_expr_sem_eval in H8; rewrite H8.
+          erewrite IHs2 by eauto.
+          simpl; trivial.
+      }
+    - {
+        Hint Constructors nnrc_imp_stmt_sem.
+        Hint Constructors nnrc_imp_stmt_sem_iter.
+        Hint Resolve nnrc_imp_stmt_sem_env_cons_same.
+        Hint Resolve nnrc_imp_stmt_sem_mcenv_cons_same.
+
+        nnrc_imp_stmt_cases (induction s) Case; simpl; intros σ₁ ψ₁ σ₂ ψ₂ sem; repeat destr sem.
+        - Case "NNRCimpSeq".
+          eauto.
+        - Case "NNRCimpLetMut".
+          invcs sem.
+          destruct p0.
+          apply nnrc_imp_expr_sem_eval in eqq.
+          eauto.
+        - Case "NNRCimpLetMut".
+          invcs sem.
+          destruct p0.
+          eauto.
+        - Case "NNRCimpBuildCollFor".
+          destruct p0; repeat destr sem; invcs sem.
+          destruct p1.
+          eauto 7.
+        - Case "NNRCimpPush".
+          invcs sem.
+          apply nnrc_imp_expr_sem_eval in eqq.
+          eauto.
+        - Case "NNRCimpAssign".
+          invcs sem.
+          apply nnrc_imp_expr_sem_eval in eqq.
+          eauto.
+        - Case "NNRCimpFor".
+          destruct d; try discriminate.
+          apply nnrc_imp_expr_sem_eval in eqq.
+          econstructor; eauto.
+          clear eqq.
+          revert σ₁ ψ₁ σ₂ ψ₂ sem.
+          induction l; intros σ₁ ψ₁ σ₂ ψ₂ sem; invcs sem; eauto 1.
+          repeat destr H0; destruct p0.
+          eauto.
+        - Case "NNRCimpIf".
+          apply nnrc_imp_expr_sem_eval in eqq.
+          destruct d; try discriminate.
+          destruct b; eauto.
+        - Case "NNRCimpEither".
+          apply nnrc_imp_expr_sem_eval in eqq.
+          destruct d; try discriminate;
+            repeat destr sem; invcs sem; destruct p0; eauto.
+      }
+  Qed.
+
+  Lemma nnrc_imp_sem_eval ret s d :
+    [ h , σc ; [ret] ⊢ s ⇓ d ] <-> [ h , σc ; [ret] ⊢〚 s 〛 ] = Some d.
+  Proof.
+    unfold nnrc_imp_stmt_eval_top_ret.
+    split; intros hyp.
+    - invcs hyp.
+      apply nnrc_imp_stmt_sem_eval in H.
+      rewrite H; trivial.
+    - destr hyp.
+      apply nnrc_imp_stmt_sem_eval in eqq.
+      destruct p; try discriminate.
+      destruct p.
+      destruct o; try discriminate.
+      invcs hyp.
+      generalize (nnrc_imp_stmt_sem_env_stack eqq).
+      simpl; intros eqq2; invcs eqq2.
+      symmetry in H1; apply domain_nil in H1; subst.
+      generalize (nnrc_imp_stmt_sem_mcenv_stack eqq).
+      simpl; intros eqq2.
+      symmetry in eqq2; apply domain_nil in eqq2; subst.
+      constructor; trivial.
+  Qed.
+  
+End NNRCimpSemEval.
